m

StandardLibrary/src/StandardLibrary.dfy
@@ -7,33 +7,31 @@ include "MemoryMath.dfy"
 module StandardLibrary {
   import opened Wrappers
   import opened U = UInt
-    // import opened MemoryMath
-
-  lemma {:axiom}XXXValueIsSafeBecauseItIsInMemory(value : nat)
-    ensures HasUint64Size(value)
-
-  lemma XXXSequenceIsSafeBecauseItIsInMemory<T>(value : seq<T>)
-    ensures HasUint64Len(value)
-  {
-    XXXValueIsSafeBecauseItIsInMemory(|value|);
-  }
-
-  function method {:opaque} XXXAdd(x : uint64, y : uint64) : (ret : uint64)
-    ensures ret as nat == x as nat + y as nat
-  {
-    XXXValueIsSafeBecauseItIsInMemory(x as nat + y as nat);
-    x + y
-  }
+  import opened MemoryMath
 
   lemma SeqTakeAppend<A>(s: seq<A>, i: int)
     requires 0 <= i < |s|
     ensures s[..i] + [s[i]] == s[..i + 1]
   {}
 
-  function method {:tailrecursion} Join<T>(ss: seq<seq<T>>, joiner: seq<T>): (s: seq<T>)
+  function Join<T>(ss: seq<seq<T>>, joiner: seq<T>): (s: seq<T>)
     requires 0 < |ss|
   {
     if |ss| == 1 then ss[0] else ss[0] + joiner + Join(ss[1..], joiner)
+  }
+  by method {
+    SequenceIsSafeBecauseItIsInMemory(ss);
+    var size := |ss| as uint64;
+    var result : seq<T>  := ss[size-1];
+    var i : uint64 := size - 1;
+    while i > 0
+      decreases i
+      invariant result == Join(ss[i..], joiner)
+    {
+      i := i - 1;
+      result := ss[i] + joiner + result;
+    }
+    return result;
   }
 
   function method {:tailrecursion} Split<T(==)>(s: seq<T>, delim: T): (res: seq<seq<T>>)
@@ -45,7 +43,7 @@ module StandardLibrary {
     decreases |s|
   {
     var i := FindIndexMatching(s, delim, 0);
-    if i.Some? then [s[..i.value]] + Split(s[XXXAdd(i.value, 1)..], delim) else [s]
+    if i.Some? then [s[..i.value]] + Split(s[Add(i.value, 1)..], delim) else [s]
   }
 
   // split on first occurrence of delim, which must exist
@@ -56,7 +54,7 @@ module StandardLibrary {
   {
     var i := FindIndexMatching(s, delim, 0);
     assert i.Some?;
-    (s[..i.value], s[XXXAdd(i.value, 1)..])
+    (s[..i.value], s[Add(i.value, 1)..])
   }
 
   // split on first occurrence of delim, return None if delim not present
@@ -66,7 +64,7 @@ module StandardLibrary {
     ensures res.Some? ==> !(delim in res.value.0)
   {
     var i :- FindIndexMatching(s, delim, 0);
-    Some((s[..i], s[XXXAdd(i, 1)..]))
+    Some((s[..i], s[Add(i, 1)..]))
   }
 
   lemma {:vcs_split_on_every_assert} WillSplitOnDelim<T>(s: seq<T>, delim: T, prefix: seq<T>)
@@ -79,7 +77,7 @@ module StandardLibrary {
       Split(s, delim);
     ==
       var i := FindIndexMatching(s, delim, 0);
-      if i.Some? then [s[..i.value]] + Split(s[XXXAdd(i.value, 1)..], delim) else [s];
+      if i.Some? then [s[..i.value]] + Split(s[Add(i.value, 1)..], delim) else [s];
     ==  { FindIndexMatchingLocatesElem(s, delim, 0, |prefix| as uint64); assert FindIndexMatching(s, delim, 0).Some?; }
       [s[..|prefix|]] + Split(s[|prefix| + 1..], delim);
     ==  { assert s[..|prefix|] == prefix; }
@@ -91,7 +89,7 @@ module StandardLibrary {
     requires delim !in s
     ensures Split(s, delim) == [s]
   {
-    XXXSequenceIsSafeBecauseItIsInMemory(s);
+    SequenceIsSafeBecauseItIsInMemory(s);
     calc {
       Split(s, delim);
     ==
@@ -125,13 +123,13 @@ module StandardLibrary {
     ensures index.None? ==> forall j :: i as nat <= j < |s| ==> !f(s[j])
     decreases |s| - i as nat
   {
-    XXXSequenceIsSafeBecauseItIsInMemory(s);
+    SequenceIsSafeBecauseItIsInMemory(s);
     if i == |s| as uint64 then None
     else if f(s[i]) then Some(i)
     else FindIndex(s, f, i + 1)
   }
 
-  function method {:tailrecursion} Filter<T>(s: seq<T>, f: T -> bool): (res: seq<T>)
+  function Filter<T>(s: seq<T>, f: T -> bool): (res: seq<T>)
     ensures forall i :: 0 <= i < |s| && f(s[i]) ==> s[i] in res
     ensures forall i :: 0 <= i < |res| ==> res[i] in s && f(res[i])
     ensures |res| <= |s|
@@ -139,6 +137,21 @@ module StandardLibrary {
     if |s| == 0 then []
     else if f(s[0]) then [s[0]] + Filter(s[1..], f)
     else Filter(s[1..], f)
+  }
+  by method {
+    SequenceIsSafeBecauseItIsInMemory(s);
+    var result : seq<T>  := [];
+    var i : uint64 := |s| as uint64;
+    while i > 0
+      decreases i
+      invariant result == Filter(s[i..], f)
+    {
+      i := i - 1;
+      if f(s[i]) {
+        result := [s[i]] + result;
+      }
+    }
+    return result;
   }
 
   lemma FilterIsDistributive<T>(s: seq<T>, s': seq<T>, f: T -> bool)
@@ -205,6 +218,8 @@ module StandardLibrary {
    *   - either:
    *      -- `a` has length `k` (that is, `a` is a prefix of `b`)
    *      -- `a[k]` is strictly less (using `less`) than `b[k]`
+   *
+   * This has ridiculously bad runtime performance, but fortunately we almost never use it
    */
 
   predicate method LexicographicLessOrEqual<T(==)>(a: seq<T>, b: seq<T>, less: (T, T) -> bool) {
@@ -352,9 +367,10 @@ module StandardLibrary {
    * SetToOrderedSequence(s, less) takes a set of T-strings and returns them as a sequence,
    * ordered by the lexicographic ordering whose underlying irreflexive ordering is "less".
    * The function is compilable, but will not exhibit enviable performance.
+   * It is ghost. ComputeSetToOrderedSequence2 should be used instead.
    */
 
-  function method {:tailrecursion} SetToOrderedSequence<T(!new,==)>(s: set<seq<T>>, less: (T, T) -> bool): (q: seq<seq<T>>)
+  function SetToOrderedSequence<T(!new,==)>(s: set<seq<T>>, less: (T, T) -> bool): (q: seq<seq<T>>)
     requires Trichotomous(less) && Transitive(less)
     ensures |s| == |q|
     ensures forall i :: 0 <= i < |q| ==> q[i] in s
